[svl] svex-reduce-with-env now has a config option. For now, it includes extensions to width-of-svex and integerp-of-svex to recognize foreign functions and recognize them when calculating width and integerp-ness of svexes (for svex-eval$).

books/centaur/svl/svex-reduce/simplify-bitand-or-xor.lisp
@@ -114,7 +114,10 @@ x
 
 (define bitand/or/xor-simple-constant-simplify (fn (arg1 svex-p)
                                                    (arg2 svex-p)
-                                                   &optional 1masked)
+                                                   &key
+                                                   (1masked 'nil)
+                                                   ((config svex-reduce-config-p)
+                                                    'config))
   ;; for easier theorem proving,
   :returns (simplified-svex sv::Svex-p :hyp (and (sv::fnsym-p fn)
                                                  (not (equal fn ':var))
@@ -190,8 +193,12 @@ x
            (bitxor-has-1 b)))
       (& (equal x 1))))
 
-  (define remove-1-from-xor ((x svex-p))
+  (define remove-1-from-xor ((x svex-p)
+                             &key
+                             ((config svex-reduce-config-p)
+                              'config))
     :returns (res svex-p :hyp (svex-p x))
+
     (case-match x
       (('sv::bitxor a b)
        (cond ((equal a 1)
@@ -209,7 +216,10 @@ x
              ))
       (& (if (equal x 1) 0 x))))
 
-  (define clear-1s-from-bitxor ((x svex-p))
+  (define clear-1s-from-bitxor ((x svex-p)
+                                &key
+                                ((config svex-reduce-config-p)
+                                 'config))
     :returns (res svex-p :hyp (svex-p x))
     (case-match x
       (('sv::bitxor a b)
@@ -240,7 +250,7 @@ x
   (
    ;; TODO: (partial) memoization can help here  to increase the limit. This may
    ;; require having a very large limit though, which might be bad again.
-   (defconst *bitand/or/xor-collect-leaves-limit* 
+   (defconst *bitand/or/xor-collect-leaves-limit*
      4))
   (case-match svex
     ((this-fn x y)
@@ -272,7 +282,8 @@ x
                                           ((limit natp) '*bitand/bitor-cancel-repeated-aux-limit*)
                                           ;;((require-integerp booleanp) 'require-integerp)
                                           ((env) 'env)
-                                          ((context rp::rp-term-listp) 'context))
+                                          ((context rp::rp-term-listp) 'context)
+                                          ((config svex-reduce-config-p) 'config))
   :verify-guards nil
   :prepwork
   (
@@ -306,7 +317,7 @@ x
          ((mv y changed-y) (bitand/bitor-cancel-repeated-aux y leaves new-val :limit (1- limit))))
       (if (or changed-x
               changed-y)
-          (mv (bitand/or/xor-simple-constant-simplify 'sv::bitor x y nil) t)
+          (mv (bitand/or/xor-simple-constant-simplify 'sv::bitor x y) t)
         (mv svex nil))))
    ((and (consp svex)
          (equal (car svex) 'sv::bitand)
@@ -316,7 +327,7 @@ x
          ((mv y changed-y) (bitand/bitor-cancel-repeated-aux y leaves new-val :limit (1- limit))))
       (if (or changed-x
               changed-y)
-          (mv (bitand/or/xor-simple-constant-simplify 'sv::bitand x y nil) t)
+          (mv (bitand/or/xor-simple-constant-simplify 'sv::bitand x y) t)
         (mv svex nil))))
    ((and (consp svex)
          (equal (car svex) 'sv::bitxor)
@@ -327,7 +338,7 @@ x
          ((Unless (and (or changed-x changed-y)
                        (integer-listp-of-svexlist leaves)))
           (mv svex nil))
-         (res (bitand/or/xor-simple-constant-simplify 'sv::bitxor new-x new-y nil))
+         (res (bitand/or/xor-simple-constant-simplify 'sv::bitxor new-x new-y))
          (res (clear-1s-from-bitxor res)))
       (mv res t)))
    (t (mv svex nil)))
@@ -370,7 +381,9 @@ x
 
   (define bitxor-remove-node ((svex svex-p)
                               (node-to-remove)
-                              (limit natp))
+                              (limit natp)
+                              &key
+                              ((config svex-reduce-config-p) 'config))
     :returns (mv (res-svex svex-p :hyp (svex-p svex))
                  success)
     ;; try to remove a node from an svex.
@@ -386,20 +399,21 @@ x
          (b* (((mv new-x success-x)
                (bitxor-remove-node x node-to-remove (1- limit)))
               ((when success-x) ;; allowed to be replaced only once.
-               (mv (bitand/or/xor-simple-constant-simplify 'sv::bitxor new-x y nil) t))
+               (mv (bitand/or/xor-simple-constant-simplify 'sv::bitxor new-x y) t))
               ((mv new-y success-y)
                (bitxor-remove-node y node-to-remove (1- limit))))
            (if success-y
-               (mv (bitand/or/xor-simple-constant-simplify 'sv::bitxor x new-y nil) t)
+               (mv (bitand/or/xor-simple-constant-simplify 'sv::bitxor x new-y) t)
              (mv svex nil))))
         (& (mv svex nil))))))
 
   (define bitxor-remove-nodes-from-both ((svex1 svex-p)
                                          (svex2 svex-p)
                                          (nodes-to-remove svexlist-p)
-                                         &optional
+                                         &key
                                          ((env) 'env)
-                                         ((context rp::rp-term-listp) 'context))
+                                         ((context rp::rp-term-listp) 'context)
+                                         ((config svex-reduce-config-p) 'config))
     :returns (mv (res-svex1 svex-p :hyp (svex-p svex1))
                  (res-svex2 svex-p :hyp (svex-p svex2)))
     ;; Try removing from both svexes at the same time.
@@ -432,7 +446,8 @@ x
                                        (y sv::svex-p)
                                        &key
                                        ((env) 'env)
-                                       ((context rp::rp-term-listp) 'context))
+                                       ((context rp::rp-term-listp) 'context)
+                                       ((config svex-reduce-config-p) 'config))
 
   :returns (simplified-svex sv::Svex-p :hyp (and (sv::fnsym-p fn)
                                                  (Not (equal fn :var))
@@ -448,7 +463,7 @@ x
           (l2 (bitand/or/xor-collect-leaves y 'sv::bitor))
           ((mv x changed-x) (bitand/bitor-cancel-repeated-aux x l2  0)))
        (if (or changed-x changed-y)
-           (bitand/or/xor-simple-constant-simplify 'sv::bitor x y nil)
+           (bitand/or/xor-simple-constant-simplify 'sv::bitor x y)
          (svex-reduce-w/-env-apply fn (hons-list x y)))))
     (sv::bitand
      (b* ((under-xor nil)
@@ -460,7 +475,7 @@ x
           ((mv x changed-x) (bitand/bitor-cancel-repeated-aux x l2  -1))
           (result
            (if (or changed-x changed-y)
-               (bitand/or/xor-simple-constant-simplify 'sv::bitand x y nil)
+               (bitand/or/xor-simple-constant-simplify 'sv::bitand x y)
              (svex-reduce-w/-env-apply fn (hons-list x y))))
           #|(- (and (bitand-xor-bad-pattern result)
           (acl2::raise "Found bitand-xor-bad-pattern. Input fn: ~p0, x:~p1, y:~p2. Result: ~p3~%" ;
@@ -478,7 +493,7 @@ x
           (rp::cwe "Some commons in botxor are found: ~p0 in x:~p1 and y:~p2~%" commons x y)))|#
           ((mv x y) (bitxor-remove-nodes-from-both x y commons))
 
-          (result (bitand/or/xor-simple-constant-simplify fn x y nil))
+          (result (bitand/or/xor-simple-constant-simplify fn x y))
 
           )
        result
@@ -520,7 +535,8 @@ x
   (define svex-simplify-bitand/or/xor ((x svex-p)
                                        &key
                                        ((env) 'env)
-                                       ((context rp::rp-term-listp) 'context))
+                                       ((context rp::rp-term-listp) 'context)
+                                       ((config svex-reduce-config-p) 'config))
     :measure (sv::svex-count x)
     :returns (res svex-p :hyp (svex-p x))
     (sv::svex-case
@@ -541,7 +557,8 @@ x
   (define svexlist-simplify-bitand/or/xor ((lst svexlist-p)
                                            &key
                                            ((env) 'env)
-                                           ((context rp::rp-term-listp) 'context))
+                                           ((context rp::rp-term-listp) 'context)
+                                           ((config svex-reduce-config-p) 'config))
     :measure (sv::svexlist-count lst)
     :returns (res svexlist-p :hyp (svexlist-p lst))
     (if (atom lst)
@@ -557,7 +574,8 @@ x
 (define svex-alist-simplify-bitand/or/xor ((alist sv::svex-alist-p)
                                            &key
                                            ((env) 'env)
-                                           ((context rp::rp-term-listp) 'context))
+                                           ((context rp::rp-term-listp) 'context)
+                                           ((config svex-reduce-config-p) 'config))
   :returns (res sv::svex-alist-p :hyp (sv::svex-alist-p alist))
   (if (atom alist)
       nil
@@ -897,8 +915,15 @@ x
                      (equal fn 'sv::bitand)
                      )
                  (svex-p arg1)
-                 (svex-p arg2))
-            (equal (svex-eval (bitand/or/xor-simple-constant-simplify fn arg1 arg2 nil)
+                 (svex-p arg2)
+
+                 (:@ :dollar-eval
+                     (width-of-svex-extn-correct<$>-lst
+                      (svex-reduce-config->width-extns config)))
+                 (:@ :normal-eval
+                     (equal (svex-reduce-config->width-extns config) nil))
+                 )
+            (equal (svex-eval (bitand/or/xor-simple-constant-simplify fn arg1 arg2)
                               env)
                    (svex-eval `(,fn ,arg1 ,arg2) env)))
    :hints (("goal"
@@ -916,7 +941,8 @@ x
                      )
                  (single-bit-4vec-p (svex-eval arg1 env))
                  (single-bit-4vec-p (svex-eval arg2 env)))
-            (equal (svex-eval (bitand/or/xor-simple-constant-simplify fn arg1 arg2 t)
+            (equal (svex-eval (bitand/or/xor-simple-constant-simplify fn arg1
+                                                                      arg2 :1masked t)
                               env)
                    (svex-eval `(,fn ,arg1 ,arg2) env)))
    :otf-flg t
@@ -961,11 +987,16 @@ x
       (implies (and
                 (sv::svexlist-p lst)
                 (rp::rp-term-listp context)
-                (integer-listp-of-svexlist lst env context)
+                (integer-listp-of-svexlist lst)
                 (rp::valid-sc env-term a)
                 (rp::eval-and-all context a)
                 (sub-alistp env big-env)
-                (rp::falist-consistent-aux big-env env-term))
+                (rp::falist-consistent-aux big-env env-term)
+                (:@ :dollar-eval
+                    (integerp-of-svex-extn-correct<$>-lst
+                     (svex-reduce-config->integerp-extns config)))
+                (:@ :normal-eval
+                    (equal (svex-reduce-config->integerp-extns config) nil)))
                (integerp (svex-eval-bitor-lst lst (rp-evlt env-term a))))
       :hints (("Goal"
                :induct (len lst)
@@ -980,7 +1011,12 @@ x
     (defthm integerp-of-svex-eval-bitor-lst-env=nil
       (implies (and
                 (sv::svexlist-p lst)
-                (integer-listp-of-svexlist lst nil context))
+                (integer-listp-of-svexlist lst :env nil)
+                (:@ :dollar-eval
+                    (integerp-of-svex-extn-correct<$>-lst
+                     (svex-reduce-config->integerp-extns config)))
+                (:@ :normal-eval
+                    (equal (svex-reduce-config->integerp-extns config) nil)))
                (integerp (svex-eval-bitor-lst lst svex-env)))
       :hints (("Goal"
                :induct (len lst)
@@ -996,11 +1032,16 @@ x
       (implies (and
                 (sv::svexlist-p lst)
                 (rp::rp-term-listp context)
-                (integer-listp-of-svexlist lst env context)
+                (integer-listp-of-svexlist lst )
                 (rp::valid-sc env-term a)
                 (rp::eval-and-all context a)
                 (sub-alistp env big-env)
-                (rp::falist-consistent-aux big-env env-term))
+                (rp::falist-consistent-aux big-env env-term)
+                (:@ :dollar-eval
+                    (integerp-of-svex-extn-correct<$>-lst
+                     (svex-reduce-config->integerp-extns config)))
+                (:@ :normal-eval
+                    (equal (svex-reduce-config->integerp-extns config) nil)))
                (integerp (svex-eval-bitand-lst lst (rp-evlt env-term a))))
       :hints (("Goal"
                :induct (len lst)
@@ -1014,7 +1055,12 @@ x
     (defthm integerp-of-svex-eval-bitand-lst-env=nil
       (implies (and
                 (sv::svexlist-p lst)
-                (integer-listp-of-svexlist lst nil context))
+                (integer-listp-of-svexlist lst :env nil)
+                (:@ :dollar-eval
+                    (integerp-of-svex-extn-correct<$>-lst
+                     (svex-reduce-config->integerp-extns config)))
+                (:@ :normal-eval
+                    (equal (svex-reduce-config->integerp-extns config) nil)))
                (integerp (svex-eval-bitand-lst lst svex-env)))
       :hints (("Goal"
                :induct (len lst)
@@ -1064,7 +1110,12 @@ x
    (svex-eval-lemma-tmpl
     (defthm svex-eval-of-clear-1s-from-bitxor-correct-lemma
       (implies (and (bitxor-has-1 x)
-                    (svex-p x))
+                    (svex-p x)
+                    (:@ :dollar-eval
+                        (width-of-svex-extn-correct<$>-lst
+                         (svex-reduce-config->width-extns config)))
+                    (:@ :normal-eval
+                        (equal (svex-reduce-config->width-extns config) nil)))
                (equal (svex-eval (remove-1-from-xor x) env)
 
                       (sv::4vec-bitxor 1
@@ -1078,7 +1129,12 @@ x
   (local
    (svex-eval-lemma-tmpl
     (defret svex-eval-of-clear-1s-from-bitxor-correct
-      (implies (svex-p x)
+      (implies (and (svex-p x)
+                    (:@ :dollar-eval
+                        (width-of-svex-extn-correct<$>-lst
+                         (svex-reduce-config->width-extns config)))
+                    (:@ :normal-eval
+                        (equal (svex-reduce-config->width-extns config) nil)))
                (equal (svex-eval res env)
                       (svex-eval x env)))
       :fn clear-1s-from-bitxor
@@ -1101,8 +1157,18 @@ x
                        (rp::eval-and-all context a)
                        (sub-alistp env big-env)
                        (rp::falist-consistent-aux big-env env-term)
+
+                       (:@ :dollar-eval
+                           (width-of-svex-extn-correct<$>-lst
+                            (svex-reduce-config->width-extns config))
+                           (integerp-of-svex-extn-correct<$>-lst
+                            (svex-reduce-config->integerp-extns config)))
+                       (:@ :normal-eval
+                           (equal (svex-reduce-config->width-extns config) nil)
+                           (equal (svex-reduce-config->integerp-extns config) nil))
+
                        )
-                  (equal
+                  (EQUAL
                    (4vec-bitor (svex-eval-bitor-lst leaves (rp-evlt env-term a))
                                (svex-eval simplified-svex (rp-evlt env-term a)))
                    (4vec-bitor (svex-eval-bitor-lst leaves (rp-evlt env-term a))
@@ -1110,7 +1176,16 @@ x
          (implies (and (equal new-val 0)
                        (svexlist-p leaves)
                        (sv::svex-p svex)
-                       (equal env nil))
+                       (equal env nil)
+
+                       (:@ :dollar-eval
+                           (width-of-svex-extn-correct<$>-lst
+                            (svex-reduce-config->width-extns config))
+                           (integerp-of-svex-extn-correct<$>-lst
+                            (svex-reduce-config->integerp-extns config)))
+                       (:@ :normal-eval
+                           (equal (svex-reduce-config->width-extns config) nil)
+                           (equal (svex-reduce-config->integerp-extns config) nil)))
                   (equal
                    (4vec-bitor (svex-eval-bitor-lst leaves svex-env)
                                (svex-eval simplified-svex svex-env))
@@ -1244,7 +1319,15 @@ x
                        (rp::valid-sc env-term a)
                        (rp::eval-and-all context a)
                        (sub-alistp env big-env)
-                       (rp::falist-consistent-aux big-env env-term))
+                       (rp::falist-consistent-aux big-env env-term)
+                       (:@ :dollar-eval
+                           (width-of-svex-extn-correct<$>-lst
+                            (svex-reduce-config->width-extns config))
+                           (integerp-of-svex-extn-correct<$>-lst
+                            (svex-reduce-config->integerp-extns config)))
+                       (:@ :normal-eval
+                           (equal (svex-reduce-config->width-extns config) nil)
+                           (equal (svex-reduce-config->integerp-extns config) nil)))
                   (equal
                    (4vec-bitand (svex-eval-bitand-lst leaves (rp-evlt env-term a))
                                 (svex-eval simplified-svex (rp-evlt env-term a)))
@@ -1253,7 +1336,15 @@ x
          (implies (and (equal new-val -1)
                        (svexlist-p leaves)
                        (sv::svex-p svex)
-                       (equal env nil))
+                       (equal env nil)
+                       (:@ :dollar-eval
+                           (width-of-svex-extn-correct<$>-lst
+                            (svex-reduce-config->width-extns config))
+                           (integerp-of-svex-extn-correct<$>-lst
+                            (svex-reduce-config->integerp-extns config)))
+                       (:@ :normal-eval
+                           (equal (svex-reduce-config->width-extns config) nil)
+                           (equal (svex-reduce-config->integerp-extns config) nil)))
                   (equal
                    (4vec-bitand (svex-eval-bitand-lst leaves svex-env)
                                 (svex-eval simplified-svex svex-env))
@@ -1391,7 +1482,15 @@ x
   (defret svex-eval-of-bitxor-remove-node-correct
     (implies (and (svex-p svex)
                   (integerp (svex-eval node-to-remove env))
-                  success)
+                  success
+                  (:@ :dollar-eval
+                      (width-of-svex-extn-correct<$>-lst
+                       (svex-reduce-config->width-extns config))
+                      (integerp-of-svex-extn-correct<$>-lst
+                       (svex-reduce-config->integerp-extns config)))
+                  (:@ :normal-eval
+                      (equal (svex-reduce-config->width-extns config) nil)
+                      (equal (svex-reduce-config->integerp-extns config) nil)))
              (equal (svex-eval res-svex env)
                     (sv::4vec-bitxor (svex-eval node-to-remove env)
                                      (svex-eval svex env))))
@@ -1414,6 +1513,15 @@ x
 
                    (sub-alistp env big-env)
                    (rp::falist-consistent-aux big-env env-term)
+
+                   (:@ :dollar-eval
+                       (width-of-svex-extn-correct<$>-lst
+                        (svex-reduce-config->width-extns config))
+                       (integerp-of-svex-extn-correct<$>-lst
+                        (svex-reduce-config->integerp-extns config)))
+                   (:@ :normal-eval
+                       (equal (svex-reduce-config->width-extns config) nil)
+                       (equal (svex-reduce-config->integerp-extns config) nil))
                    )
               (equal (sv::4vec-bitxor (svex-eval res-svex1 (rp-evlt env-term a))
                                       (svex-eval res-svex2 (rp-evlt env-term a)))
@@ -1424,6 +1532,15 @@ x
                    (svexlist-p nodes-to-remove)
 
                    (equal env nil)
+
+                   (:@ :dollar-eval
+                       (width-of-svex-extn-correct<$>-lst
+                        (svex-reduce-config->width-extns config))
+                       (integerp-of-svex-extn-correct<$>-lst
+                        (svex-reduce-config->integerp-extns config)))
+                   (:@ :normal-eval
+                       (equal (svex-reduce-config->width-extns config) nil)
+                       (equal (svex-reduce-config->integerp-extns config) nil))
                    )
               (equal (sv::4vec-bitxor (svex-eval res-svex1 svex-env)
                                       (svex-eval res-svex2 svex-env))
@@ -1469,7 +1586,15 @@ x
                       (rp::valid-sc env-term a)
                       (rp::eval-and-all context a)
                       (sub-alistp env big-env)
-                      (rp::falist-consistent-aux big-env env-term))
+                      (rp::falist-consistent-aux big-env env-term)
+                      (:@ :dollar-eval
+                          (width-of-svex-extn-correct<$>-lst
+                           (svex-reduce-config->width-extns config))
+                          (integerp-of-svex-extn-correct<$>-lst
+                           (svex-reduce-config->integerp-extns config)))
+                      (:@ :normal-eval
+                          (equal (svex-reduce-config->width-extns config) nil)
+                          (equal (svex-reduce-config->integerp-extns config) nil)))
                  (equal
                   (svex-eval simplified-svex (rp-evlt env-term a))
                   (svex-eval `(,fn ,x ,y) (rp-evlt env-term a))))
@@ -1538,7 +1663,15 @@ x
    (implies (and* (fnsym-p fn)
                   (sv::svex-p x)
                   (sv::svex-p y)
-                  (equal env nil))
+                  (equal env nil)
+                  (:@ :dollar-eval
+                      (width-of-svex-extn-correct<$>-lst
+                       (svex-reduce-config->width-extns config))
+                      (integerp-of-svex-extn-correct<$>-lst
+                       (svex-reduce-config->integerp-extns config)))
+                  (:@ :normal-eval
+                      (equal (svex-reduce-config->width-extns config) nil)
+                      (equal (svex-reduce-config->integerp-extns config) nil)))
             (equal
              (svex-eval simplified-svex svex-env)
              (svex-eval `(,fn ,x ,y) svex-env)))
@@ -1608,7 +1741,15 @@ x
                    (rp::valid-sc env-term a)
                    (rp::eval-and-all context a)
                    (sub-alistp env big-env)
-                   (rp::falist-consistent-aux big-env env-term))
+                   (rp::falist-consistent-aux big-env env-term)
+                   (:@ :dollar-eval
+                       (width-of-svex-extn-correct<$>-lst
+                        (svex-reduce-config->width-extns config))
+                       (integerp-of-svex-extn-correct<$>-lst
+                        (svex-reduce-config->integerp-extns config)))
+                   (:@ :normal-eval
+                       (equal (svex-reduce-config->width-extns config) nil)
+                       (equal (svex-reduce-config->integerp-extns config) nil)))
               (equal
                (svex-eval res (rp-evlt env-term a))
                (svex-eval x (rp-evlt env-term a))))
@@ -1619,7 +1760,15 @@ x
                    (rp::valid-sc env-term a)
                    (rp::eval-and-all context a)
                    (sub-alistp env big-env)
-                   (rp::falist-consistent-aux big-env env-term))
+                   (rp::falist-consistent-aux big-env env-term)
+                   (:@ :dollar-eval
+                       (width-of-svex-extn-correct<$>-lst
+                        (svex-reduce-config->width-extns config))
+                       (integerp-of-svex-extn-correct<$>-lst
+                        (svex-reduce-config->integerp-extns config)))
+                   (:@ :normal-eval
+                       (equal (svex-reduce-config->width-extns config) nil)
+                       (equal (svex-reduce-config->integerp-extns config) nil)))
               (equal
                (svexlist-eval res (rp-evlt env-term a))
                (svexlist-eval lst (rp-evlt env-term a))))
@@ -1640,14 +1789,30 @@ x
  (defret-mutual svex-eval-of-<fn>
    (defret svex-eval-of-<fn>-env=nil
      (implies (and (sv::svex-p x)
-                   (equal env nil))
+                   (equal env nil)
+                   (:@ :dollar-eval
+                       (width-of-svex-extn-correct<$>-lst
+                        (svex-reduce-config->width-extns config))
+                       (integerp-of-svex-extn-correct<$>-lst
+                        (svex-reduce-config->integerp-extns config)))
+                   (:@ :normal-eval
+                       (equal (svex-reduce-config->width-extns config) nil)
+                       (equal (svex-reduce-config->integerp-extns config) nil)))
               (equal
                (svex-eval res svex-env)
                (svex-eval x svex-env)))
      :fn svex-simplify-bitand/or/xor)
    (defret svexlist-eval-of-<fn>-env=nil
      (implies (and (sv::svexlist-p lst)
-                   (equal env nil))
+                   (equal env nil)
+                   (:@ :dollar-eval
+                       (width-of-svex-extn-correct<$>-lst
+                        (svex-reduce-config->width-extns config))
+                       (integerp-of-svex-extn-correct<$>-lst
+                        (svex-reduce-config->integerp-extns config)))
+                   (:@ :normal-eval
+                       (equal (svex-reduce-config->width-extns config) nil)
+                       (equal (svex-reduce-config->integerp-extns config) nil)))
               (equal
                (svexlist-eval res svex-env)
                (svexlist-eval lst svex-env)))
@@ -1672,7 +1837,15 @@ x
                  (rp::eval-and-all context a)
 
                  (sub-alistp env big-env)
-                 (rp::falist-consistent-aux big-env env-term))
+                 (rp::falist-consistent-aux big-env env-term)
+                 (:@ :dollar-eval
+                     (width-of-svex-extn-correct<$>-lst
+                      (svex-reduce-config->width-extns config))
+                     (integerp-of-svex-extn-correct<$>-lst
+                      (svex-reduce-config->integerp-extns config)))
+                 (:@ :normal-eval
+                     (equal (svex-reduce-config->width-extns config) nil)
+                     (equal (svex-reduce-config->integerp-extns config) nil)))
             (equal
              (svex-alist-eval res (rp-evlt env-term a))
              (svex-alist-eval alist (rp-evlt env-term a))))
@@ -1685,7 +1858,15 @@ x
 (svex-eval-lemma-tmpl
  (defret svex-alist-eval-of-<fn>=env=nil
    (implies (and (sv::svex-alist-p alist)
-                 (equal env nil))
+                 (equal env nil)
+                 (:@ :dollar-eval
+                     (width-of-svex-extn-correct<$>-lst
+                      (svex-reduce-config->width-extns config))
+                     (integerp-of-svex-extn-correct<$>-lst
+                      (svex-reduce-config->integerp-extns config)))
+                 (:@ :normal-eval
+                     (equal (svex-reduce-config->width-extns config) nil)
+                     (equal (svex-reduce-config->integerp-extns config) nil)))
             (equal
              (svex-alist-eval res svex-env)
              (svex-alist-eval alist svex-env)))
