books/centaur/svl/svex-reduce/base.lisp
@@ -39,22 +39,333 @@
                         nil)))
     nil))
 
-(DEFMACRO hons-LIST (&REST ARGS)
+(DEFMACRO hons-list (&REST ARGS)
   (hons-list-macro ARGS))
 
 (defmacro svex-eval-lemma-tmpl (form)
   `(progn
-     ,form
      ,(acl2::template-subst
        form
+       :features '(:normal-eval)
+       :str-alist '(("<$>" . ""))
+       :pkg-sym 'pkg
+       )
+     ,(acl2::template-subst
+       form
+       :features '(:dollar-eval)
        :atom-alist '((svex-eval . svex-eval$)
                      (svex-apply . svex-apply$)
                      (svexlist-eval . svexlist-eval$)
                      (svex-alist-eval . svex-alist-eval$))
-       :str-alist '(("SVEX-EVAL" . "SVEX-EVAL$")
+       :str-alist '(("<$>" . "$")
+                    ("SVEX-EVAL" . "SVEX-EVAL$")
                     ("SVEX-APPLY" . "SVEX-APPLY$")
                     ("SVEXLIST-EVAL" . "SVEXLIST-EVAL$")
                     ("SVEX-ALIST-EVAL" . "SVEX-ALIST-EVAL$"))
        :pkg-sym 'pkg
        )
      ))
+
+(defsection integerp-of-svex-extn
+
+  (define svex-foreign-fnsym-p (fn)
+    (and (sv::fnsym-p fn)
+         (not (assoc-equal fn
+                           sv::*svex-op-table*)))
+    ///
+    (define svex-foreign-fnsym-fix ((x svex-foreign-fnsym-p))
+      :enabled t
+      (mbe :exec x
+           :logic (if (svex-foreign-fnsym-p x) x 'identity)))
+    (local
+     (in-theory (enable svex-foreign-fnsym-fix)))
+    (fty::deffixtype svex-foreign-fnsym
+      :pred svex-foreign-fnsym-p
+      :fix svex-foreign-fnsym-fix
+      :equiv svex-foreign-fnsym-equiv
+      :define t))
+
+  (fty::defprod integerp-of-svex-extn
+    ((fn svex-foreign-fnsym)
+     (arg-len posp :rule-classes (:rewrite :type-prescription)))
+    :layout :fulltree)
+
+  (fty::deflist integerp-of-svex-extn-list
+    :elt-type integerp-of-svex-extn
+    :true-listp t
+    )
+
+  (defthm integerp-of-svex-extn-listp-is-alist-p
+    (implies (integerp-of-svex-extn-list-p lst)
+             (alistp lst))
+    :rule-classes (:rewrite :forward-chaining :type-prescription))
+
+  (svex-eval-lemma-tmpl
+   (defun-sk integerp-of-svex-extn-correct<$> (obj)
+     ;;(declare (xargs :guard (integerp-of-svex-extn-p obj)))
+     (forall (args env)
+             (b* (((integerp-of-svex-extn obj)))
+               (implies (and (equal (len args) obj.arg-len)
+                             (integer-listp (svexlist-eval args env)))
+                        (integerp (svex-eval `(,obj.fn . ,args) env)))))))
+
+  (svex-eval-lemma-tmpl
+   (defun integerp-of-svex-extn-correct<$>-lst (lst)
+     (if (atom lst)
+         (equal lst nil)
+       (and (integerp-of-svex-extn-correct<$> (car lst))
+            (integerp-of-svex-extn-correct<$>-lst (cdr lst))))))
+
+  ;; (define ha-s (x y)
+  ;;   :verify-guards nil
+  ;;   :returns (res integerp :hyp (and (integerp x)
+  ;;                                    (integerp y)))
+  ;;   (sv::4vec-bitxor x y)
+  ;;   ///
+  ;;   (defwarrant ha-s))
+
+  ;; (local
+  ;;  (defthm equal-of-len-with-contant
+  ;;    (implies (and (syntaxp (quotep c))
+  ;;                  (posp c))
+  ;;             (equal (equal (len x) c)
+  ;;                    (and (consp x)
+  ;;                         (equal (len (cdr x)) (1- c)))))))
+
+  ;; (defthm integerp-of-svex-extn-for-ha-s-correct
+  ;;   (implies (APPLY$-WARRANT-HA-S)
+  ;;            (integerp-of-svex-extn-correct$ 'ha-s 2))
+  ;;   :hints (("Goal"
+  ;;            :do-not-induct t
+  ;;            :in-theory (e/d (ha-s
+  ;;                             SVEX-EVAL$
+  ;;                             svex-kind
+  ;;                             SVEX-CALL->FN
+  ;;                             SVEX-CALL->ARGS
+  ;;                             SVEXLIST-EVAL$
+  ;;                             svex-apply$)
+  ;;                            (RP::DUMMY-LEN-EQUIV
+  ;;                             len)))))
+  )
+
+(defsection width-of-svex-extn
+
+  #!acl2
+  (local (flag::make-flag all-vars1-flag all-vars1))
+  #!acl2
+  (local (defthm-all-vars1-flag
+           (defthm true-listp-of-all-vars1
+             (implies (true-listp ans)
+                      (true-listp (all-vars1 term ans)))
+             :hints ('(:expand ((all-vars1 term ans))))
+             :flag all-vars1)
+           (defthm true-listp-of-all-vars1-lst
+             (implies (true-listp ans)
+                      (true-listp (all-vars1-lst lst ans)))
+             :hints ('(:expand ((all-vars1-lst lst ans))))
+             :flag all-vars1-lst)))
+
+  #!acl2(defthm true-listp-of-all-fnnames1-type
+          (implies (true-listp acc)
+                   (true-listp (all-fnnames1 flg x acc)))
+          :rule-classes :type-prescription)
+
+  (local
+   (in-theory (disable acl2::all-vars1
+                       acl2::all-fnnames1
+                       subsetp-equal)))
+
+  (define safe-max (x y)
+    (and (natp x)
+         (natp y)
+         (max x y)))
+
+  (define safe-min (x y)
+    (and (natp x)
+         (natp y)
+         (min x y)))
+
+  (define width-of-svex-extn-formula-p (x)
+    (and (pseudo-termp x)
+         (subsetp-equal
+          (acl2::all-fnnames x)
+          '(safe-max safe-min nth))
+         (subsetp-equal
+          (acl2::all-vars x)
+          '(widths)))
+    ///
+    (define width-of-svex-extn-formula-fix ((x width-of-svex-extn-formula-p))
+      :enabled t
+      (mbe :exec x
+           :logic (if (width-of-svex-extn-formula-p x) x ''nil)))
+    (local
+     (in-theory (enable width-of-svex-extn-formula-fix)))
+    (fty::deffixtype width-of-svex-extn-formula
+      :pred width-of-svex-extn-formula-p
+      :fix width-of-svex-extn-formula-fix
+      :equiv width-of-svex-extn-formula-equiv
+      :define t))
+
+  (fty::defprod width-of-svex-extn
+    ((fn svex-foreign-fnsym)
+     (arg-len posp :rule-classes (:rewrite :type-prescription))
+     (formula width-of-svex-extn-formula)
+     )
+    :layout :fulltree)
+
+  (fty::deflist width-of-svex-extn-list
+    :elt-type width-of-svex-extn
+    :true-listp t
+    )
+
+  #|(define maybe-nat-listp (lst)
+  (if (atom lst)
+  (equal lst nil)
+  (and (acl2::maybe-natp (car lst))
+  (maybe-nat-listp (cdr lst)))))|#
+
+  (define 4vec-correct-width-p (width val)
+    :verify-guards nil
+    (implies (natp width)
+             (equal (4vec-part-select 0 width val)
+                    val)))
+
+  (define 4vec-correct-widths-p (widths vals )
+    :verify-guards nil
+    (if (or (atom widths)
+            (atom vals))
+        (and (equal widths nil)
+             (equal vals nil))
+      (and (4vec-correct-width-p (car widths)
+                                 (car vals))
+           (4vec-correct-widths-p (cdr widths)
+                                  (cdr vals)))))
+
+
+  (define width-of-svex-extn-formula-eval ((formula)
+                                           (widths true-listp))
+    :guard-hints (("Goal"
+                   :in-theory (e/d (width-of-svex-extn-formula-p) ())))
+    (cond ((atom widths)
+           (list 'quote widths))
+          ((and (quotep formula)
+                (consp (cdr formula)))
+           (unquote formula))
+          (t (case-match formula
+               (('safe-max a b)
+                (b* ((a (width-of-svex-extn-formula-eval a widths))
+                     (b (width-of-svex-extn-formula-eval b widths)))
+                  (safe-max a b)))
+               (('safe-min a b)
+                (b* ((a (width-of-svex-extn-formula-eval a widths))
+                     (b (width-of-svex-extn-formula-eval b widths)))
+                  (safe-min a b)))
+               (('nth a 'widths)
+                (b* ((a (nfix (width-of-svex-extn-formula-eval a widths))))
+                  (nth a widths)))
+               (&
+                (acl2::raise
+                 "Formula is in unsupported format: ~p0" formula))
+               ))))
+
+  (defun-sk width-of-svex-extn-correct$ (obj)
+    ;;(declare (xargs :guard (width-of-svex-extn-p obj)))
+    (forall
+     (args widths env)
+     (b* (((width-of-svex-extn obj) obj))
+       (implies (and (equal (len args) obj.arg-len)
+                     (equal (len widths) obj.arg-len)
+                     (4vec-correct-widths-p widths
+                                            (svexlist-eval$ args env)))
+                (4vec-correct-width-p
+                 (width-of-svex-extn-formula-eval obj.formula
+                                                  widths)
+                 (svex-eval$ (sv::svex-call obj.fn args)
+                             env))))))
+
+  (defun width-of-svex-extn-correct$-lst (lst)
+    (if (atom lst)
+        (equal lst nil)
+      (and (width-of-svex-extn-correct$ (car lst))
+           (width-of-svex-extn-correct$-lst (cdr lst)))))
+
+  )
+
+;; (INCLUDE-BOOK "projects/apply/top" :DIR :SYSTEM)
+
+;; (define ha-s (x y)
+;;   :verify-guards nil
+;;   (sv::4vec-bitxor x y)
+;;   ///
+;;   (defwarrant ha-s))
+
+;; (local
+;;  (defthm equal-of-len-with-constant
+;;    (implies (and (syntaxp (quotep c))
+;;                  (posp c))
+;;             (equal (equal (len x) c)
+;;                    (and (consp x)
+;;                         (equal (len (cdr x)) (1- c)))))))
+
+;; (defconst *ha-s-width-formula*
+;;   '(safe-max (nth '0 widths)
+;;              (nth '1 widths)))
+
+;; (include-book "../4vec-lemmas")
+
+;; (defthm 4VEC-CORRECT-WIDTH-P-of-not-natp
+;;   (implies (not (natp width))
+;;            (4VEC-CORRECT-WIDTH-P width x))
+;;   :hints (("Goal"
+;;            :in-theory (e/d (4VEC-CORRECT-WIDTH-P) ()))))
+
+;; (skip-proofs
+;;  (defthm 4VEC-CORRECT-WIDTH-P-of-4VEC-BITXOR
+;;   (implies (and (4VEC-CORRECT-WIDTH-P w1 a1)
+;;                 (4VEC-CORRECT-WIDTH-P w2 a2))
+;;            (4VEC-CORRECT-WIDTH-P (safe-max w1 w2)
+;;                                  (sv::4vec-bitxor a1 a2)))
+;;   :hints (("Goal"
+;;            :in-theory (e/d (4VEC-CORRECT-WIDTH-P
+;;                             4vec-part-select-of-4vec-bitxor-better
+;;                             safe-max)
+;;                            ())))))
+
+;; (defthm width-of-svex-extn-correct$-of-ha-s
+;;   (b* ((obj (make-width-of-svex-extn
+;;              :fn 'ha-s
+;;              :arg-len 2
+;;              :formula *ha-s-width-formula*)))
+;;     (implies (APPLY$-WARRANT-HA-S)
+;;              (width-of-svex-extn-correct$ obj)))
+;;   :hints (("Goal"
+;;            :in-theory (e/d (4VEC-CORRECT-WIDTHS-P
+;;                             ;;4VEC-CORRECT-WIDTH-P
+;;                             ;;SAFE-MAX
+;;                             nth
+;;                             SVEXLIST-EVAL$
+;;                             ;;SVEX-EVAL$-CORRECT-WIDTHS-P
+;;                             ;;SVEX-EVAL$-CORRECT-WIDTH-P
+;;                             SVEX-EVAL$
+;;                             svex-kind
+;;                             ;;SVEX-CALL->ARGS
+;;                             ;;SVEX-CALL->fn
+;;                             SVEX-APPLY$
+;;                             HA-S
+;;                             ;;SAFE-MAX
+;;                             4vec-part-select-of-4vec-bitxor-better
+;;                             WIDTH-OF-SVEX-EXTN-FORMULA-EVAL)
+;;                            (;;nth
+;;                             natp)))))
+
+
+
+;;;;
+
+
+
+(fty::defprod svex-reduce-config
+  ((width-extns width-of-svex-extn-list)
+   (integerp-extns integerp-of-svex-extn-list) )
+  :layout :tree
+  )
