books/centaur/svl/svex-reduce/width-of-svex.lisp
@@ -66,147 +66,189 @@
   use-equal-by-logbitp
   :disabled t))
 
-(define width-of-svex ((x sv::svex-p))
-  :returns (width acl2::maybe-natp)
-  :measure (sv::Svex-count x)
-  (sv::svex-case
-   x
-   :var nil
-   :quote (cond ((natp x)
-                 (integer-length x))
-                ((4vec-p x)
-                 (b* (((4vec x)))
-                   (and (natp x.upper)
-                        (natp x.lower)
-                        (max (integer-length x.upper)
-                             (integer-length x.lower))))))
-   :call
-   (cond ((and* (equal x.fn 'sv::bitand)
-                (equal-len x.args 2))
-          (b* ((w1 (width-of-svex (first x.args)))
-               (w2 (width-of-svex (second x.args)))
-               ((Unless w1) w2)
-               ((unless w2) w1))
-            (min w1 w2)))
-         ((and* (or (equal x.fn 'sv::bitor)
-                    (equal x.fn 'sv::bitxor)
-                    (equal x.fn 'sv::res))
-                (equal-len x.args 2))
-          (b* ((w1 (width-of-svex (first x.args)))
-               ((Unless w1) nil)
-               (w2 (width-of-svex (second x.args)))
-               ((Unless w2) nil))
-            (max w1 w2)))
-         ((and* (equal x.fn 'sv::partsel)
-                (equal-len x.args 3))
-          ;; TODO: An option to do further search here can be implemented to see if
-          ;; the argument of partsel is even narrower than its size indicates..
-          (b* ((start (first x.args))
-               (size (second x.args)))
-            (and (natp start)
-                 (natp size)
-                 size)))
-         ((and* (equal x.fn 'sv::concat)
-                (equal-len x.args 3))
-          (b* ((size (first x.args))
-               ((Unless (natp size)) nil)
-               (term1 (second x.args))
-               (term2 (third x.args))
-               (term2-width (width-of-svex term2))
-               ((Unless term2-width)
-                nil)
-               ((unless (equal term2-width 0))
-                (+ size term2-width))
-               (term1-size (width-of-svex term1)))
-            (if term1-size
-                (min size term1-size)
-              size)))
+(defines width-of-svex
+  :flag-local nil
+  (define width-of-svex ((x sv::svex-p)
+                         &key
+                         ((config svex-reduce-config-p)
+                          'config))
+    :returns (width acl2::maybe-natp)
+    :measure (sv::svex-count x)
+    :verify-guards nil
+    (sv::svex-case
+     x
+     :var nil
+     :quote (cond ((natp x)
+                   (integer-length x))
+                  ((4vec-p x)
+                   (b* (((4vec x)))
+                     (and (natp x.upper)
+                          (natp x.lower)
+                          (max (integer-length x.upper)
+                               (integer-length x.lower))))))
+     :call
+     (cond ((and* (equal x.fn 'sv::bitand)
+                  (equal-len x.args 2))
+            (b* ((w1 (width-of-svex (first x.args)))
+                 (w2 (width-of-svex (second x.args)))
+                 ((Unless w1) w2)
+                 ((unless w2) w1))
+              (min w1 w2)))
+           ((and* (or* (equal x.fn 'sv::bitor)
+                       (equal x.fn 'sv::bitxor)
+                       (equal x.fn 'sv::res))
+                  (equal-len x.args 2))
+            (b* ((w1 (width-of-svex (first x.args)))
+                 ((Unless w1) nil)
+                 (w2 (width-of-svex (second x.args)))
+                 ((Unless w2) nil))
+              (max w1 w2)))
+           ((and* (equal x.fn 'sv::partsel)
+                  (equal-len x.args 3))
+            ;; TODO: An option to do further search here can be implemented to see if
+            ;; the argument of partsel is even narrower than its size indicates..
+            (b* ((start (first x.args))
+                 (size (second x.args)))
+              (and (natp start)
+                   (natp size)
+                   size)))
+           ((and* (equal x.fn 'sv::concat)
+                  (equal-len x.args 3))
+            (b* ((size (first x.args))
+                 ((Unless (natp size)) nil)
+                 (term1 (second x.args))
+                 (term2 (third x.args))
+                 (term2-width (width-of-svex term2))
+                 ((Unless term2-width)
+                  nil)
+                 ((unless (equal term2-width 0))
+                  (+ size term2-width))
+                 (term1-size (width-of-svex term1)))
+              (if term1-size
+                  (min size term1-size)
+                size)))
 
-         ((and* (equal x.fn 'sv::zerox)
-                (equal-len x.args 2))
-          (b* ((size (first x.args))
-               ((Unless (natp size)) nil)
-               (term1 (second x.args))
-               (term1-size (width-of-svex term1)))
-            (if term1-size
-                (min size (width-of-svex term1))
-              size)))
+           ((and* (equal x.fn 'sv::zerox)
+                  (equal-len x.args 2))
+            (b* ((size (first x.args))
+                 ((Unless (natp size)) nil)
+                 (term1 (second x.args))
+                 (term1-size (width-of-svex term1)))
+              (if term1-size
+                  (min size (width-of-svex term1))
+                size)))
 
-         ((and* (or (equal x.fn 'sv::unfloat)
-                    (equal x.fn 'sv::id))
-                (equal-len x.args 1))
-          (width-of-svex (first x.args)))
+           ((and* (or* (equal x.fn 'sv::unfloat)
+                       (equal x.fn 'sv::id))
+                  (equal-len x.args 1))
+            (width-of-svex (first x.args)))
 
-         ((and* (equal x.fn 'sv::lsh)
-                (equal-len x.args 2))
-          (b* ((size (first x.args))
-               ((Unless (natp size)) nil)
-               (term1 (second x.args))
-               (term1-size (width-of-svex term1)))
-            (and term1-size
-                 (+ term1-size size))))
+           ((and* (equal x.fn 'sv::lsh)
+                  (equal-len x.args 2))
+            (b* ((size (first x.args))
+                 ((Unless (natp size)) nil)
+                 (term1 (second x.args))
+                 (term1-size (width-of-svex term1)))
+              (and term1-size
+                   (+ term1-size size))))
 
-         ((and* (equal x.fn 'sv::rsh)
-                (equal-len x.args 2))
-          (b* ((size (first x.args))
-               ((Unless (natp size)) nil)
-               (term1 (second x.args))
-               (term1-size (width-of-svex term1)))
-            (and term1-size
-                 (nfix (+ term1-size (- size))))))
+           ((and* (equal x.fn 'sv::rsh)
+                  (equal-len x.args 2))
+            (b* ((size (first x.args))
+                 ((Unless (natp size)) nil)
+                 (term1 (second x.args))
+                 (term1-size (width-of-svex term1)))
+              (and term1-size
+                   (nfix (+ term1-size (- size))))))
 
-         ((and* (or (equal x.fn 'sv::?!)
-                    (equal x.fn 'sv::?)
-                    (equal x.fn 'sv::?*)
-                    (equal x.fn 'sv::bit?!)
-                    (equal x.fn 'sv::bit?))
-                (equal-len x.args 3))
-          (b* (
-               (w1 (width-of-svex (second x.args)))
-               ((Unless w1) nil)
-               (w2 (width-of-svex (third x.args)))
-               ((Unless w2) nil))
-            (max w1 w2)))
+           ((and* (or* (equal x.fn 'sv::?!)
+                       (equal x.fn 'sv::?)
+                       (equal x.fn 'sv::?*)
+                       (equal x.fn 'sv::bit?!)
+                       (equal x.fn 'sv::bit?))
+                  (equal-len x.args 3))
+            (b* ((w1 (width-of-svex (second x.args)))
+                 ((Unless w1) nil)
+                 (w2 (width-of-svex (third x.args)))
+                 ((Unless w2) nil))
+              (max w1 w2)))
 
-         #|((and* (equal x.fn 'sv::partinst)
-         (equal-len x.args 4)) ;
-         ;; I don't expect to get partinst here for my use case. So I am not ;
-         going to try to prove this here. ;
-; ; ;
-         ;; TODO: there  could be made  a slight improvement here  by checking ;
-         ;; new-val's acutal size as well. (+ start new-val-size) can be added ;
-         ;; into  the  final  calculation.  If  (+  start  size)  is  >=  than ;
-         ;; old-val-width,  then   min  of  (+   start  size)  and   (+  start ;
-         ;; new-val-size) can be picked. ;
-         (b* ((start (first x.args)) ;
-         (size (second x.args)) ;
-         ((unless (and (natp start) ;
-         (natp size))) ;
-         nil) ;
-         (old-val (third x.args)) ;
-         (?new-val (fourth x.args)) ;
-         (old-val-width (width-of-svex old-val)) ;
-         ((unless old-val-width) ;
-         nil)) ;
-         (max (+ start size) old-val-width)))|#
+           (t (b* (((svex-reduce-config config) config)
+                   (obj (assoc-equal x.fn config.width-extns))
+                   ((unless obj) nil)
+                   ((width-of-svex-extn obj) obj)
+                   ((unless (equal (len x.args) obj.arg-len))
+                    nil)
+                   ((Unless (mbt (posp obj.arg-len))) nil) ;; for measure
+                   ((Unless (mbt (width-of-svex-extn-p obj)))
+                    nil) ;; for proofs without this hyp.
+                   (widths (widths-of-svexlist x.args))
+                   (res (width-of-svex-extn-formula-eval obj.formula widths)))
+                (and (natp res)
+                     res)))
 
-         )))
+           #|((and* (equal x.fn 'sv::partinst)
+           (equal-len x.args 4)) ; ; ;
+           ;; I don't expect to get partinst here for my use case. So I am not ; ; ;
+           going to try to prove this here. ; ; ;
+; ; ; ; ; ; ; ; ; ; ; ; ; ; ;
+           ;; TODO: there  could be made  a slight improvement here  by checking ; ; ;
+           ;; new-val's acutal size as well. (+ start new-val-size) can be added ; ; ;
+           ;; into  the  final  calculation.  If  (+  start  size)  is  >=  than ; ; ;
+           ;; old-val-width,  then   min  of  (+   start  size)  and   (+  start ; ; ;
+           ;; new-val-size) can be picked. ; ; ;
+           (b* ((start (first x.args)) ; ; ;
+           (size (second x.args)) ; ; ;
+           ((unless (and (natp start) ; ; ;
+           (natp size))) ; ; ;
+           nil) ; ; ;
+           (old-val (third x.args)) ; ; ;
+           (?new-val (fourth x.args)) ; ; ;
+           (old-val-width (width-of-svex old-val)) ; ; ;
+           ((unless old-val-width) ; ; ;
+           nil)) ; ; ;
+           (max (+ start size) old-val-width)))|#
+
+           )))
+  (define widths-of-svexlist ((lst sv::svexlist-p)
+                              &key
+                              ((config svex-reduce-config-p)
+                               'config))
+    :returns (widths)
+    :measure (sv::svexlist-count lst)
+    (if (atom lst)
+        nil
+      (cons (width-of-svex (car lst))
+            (widths-of-svexlist (cdr lst))))))
+
+(local
+ (defthm width-of-svex-extn-p-of-assoc-equal
+   (implies (and (assoc-equal fn WIDTH-EXTNS)
+                 (WIDTH-OF-SVEX-EXTN-list-P WIDTH-EXTNS))
+            (width-of-svex-extn-p (ASSOC-EQUAL fn WIDTH-EXTNS)))))
+
+(local
+ (defthm alistp-of-WIDTH-OF-SVEX-EXTN-list-P
+   (implies (width-of-svex-extn-list-p x)
+            (alistp x))))
+
+(verify-guards width-of-svex-fn)
 
 ;; maybe better to memoize for only a handful of svex functions..
 (memoize 'width-of-svex
          :condition '(and (equal (svex-kind x) :call)
-                          (member-equal (svex-call->fn x)
-                                        '(sv::bitor
-                                          sv::concat
-                                          sv::bitxor
-                                          sv::bitand
-                                          sv::?!
-                                          sv::?
-                                          sv::?*
-                                          sv::bit?!
-                                          sv::bit?
-                                          sv::rsh
-                                          sv::lsh)))
+                          #|(member-equal (svex-call->fn x)
+                          '(sv::bitor
+                          sv::concat
+                          sv::bitxor
+                          sv::bitand
+                          sv::?!
+                          sv::?
+                          sv::?*
+                          sv::bit?!
+                          sv::bit?
+                          sv::rsh
+                          sv::lsh))|#)
          )
 
 (local
@@ -294,13 +336,54 @@
                               4vec-concat)
                              (BITOPS::LOGHEAD-OF-LOGAND))))))
 
+
+(defthm 4vec-correct-width-p-of-4vec-bitxor
+  (implies (and ;;(natp w1)
+                ;;(natp w2)
+                (4vec-correct-width-p w1 a1)
+                (4vec-correct-width-p w2 a2)
+                (equal w (safe-max w1 w2)))
+           (4vec-correct-width-p w (sv::4vec-bitxor a1 a2)))
+  :hints (("goal"
+           :in-theory (e/d (natp
+                            4vec-correct-width-p
+                            4vec-part-select-of-4vec-bitxor-better
+                            safe-max)
+                           ()))))
+
+(defthm 4vec-correct-width-p-of-4vec-bitor
+  (implies (and ;;(natp w1)
+                ;;(natp w2)
+                (4vec-correct-width-p w1 a1)
+                (4vec-correct-width-p w2 a2)
+                (equal w (safe-max w1 w2)))
+           (4vec-correct-width-p w (sv::4vec-bitor a1 a2)))
+  :hints (("goal"
+           :in-theory (e/d (4vec-correct-width-p
+                            4vec-part-select-of-4vec-bitor-better
+                            safe-max)
+                           ()))))
+
+(defthm 4vec-correct-width-p-of-4vec-bitand
+  (implies (and ;;(natp w1)
+                ;;(natp w2)
+                (4vec-correct-width-p w1 a1)
+                (4vec-correct-width-p w2 a2)
+                (equal w (safe-min w1 w2)))
+           (4vec-correct-width-p w (sv::4vec-bitand a1 a2)))
+  :hints (("goal"
+           :in-theory (e/d (4vec-correct-width-p
+                            4vec-part-select-of-4vec-bitand-better
+                            safe-min)
+                           ()))))
+
 (local
  (svex-eval-lemma-tmpl
   (defthm svex-eval-when-svex-is-natp
-   (implies (natp x)
-            (equal (svex-eval x env) x))
-   :hints (("Goal"
-            :in-theory (e/d (svex-eval svex-kind SV::SVEX-QUOTE->VAL) ()))))))
+    (implies (natp x)
+             (equal (svex-eval x env) x))
+    :hints (("Goal"
+             :in-theory (e/d (svex-eval svex-kind SV::SVEX-QUOTE->VAL) ()))))))
 
 (local
  (defthm 4vec-concat-of-0-is-4vec-part-select
@@ -385,60 +468,273 @@
    (implies (and (natp lsb)
                  (natp width))
             (equal (equal x (4vec-part-install lsb width in val))
-                   (equal x (4VEC-CONCAT
+                   (equal x (4vec-concat
                              lsb in
-                             (4VEC-CONCAT
+                             (4vec-concat
                               width val
-                              (4VEC-RSH (+ lsb width) in))))))
-   :hints (("Goal"
-            :in-theory (e/d (2VEC
-                             4VEC
+                              (4vec-rsh (+ lsb width) in))))))
+   :hints (("goal"
+            :in-theory (e/d (2vec
+                             4vec
                              4vec-part-install) ())))))
 
 (local
  (in-theory (disable sv::svex-apply$-is-svex-apply)))
 
-(svex-eval-lemma-tmpl
- (defret svex-eval-<fn>-is-correct-1
-  (implies (and width
-                (sv::Svex-p x))
-           (equal (4vec-part-select 0 width (svex-eval x env))
-                  (svex-eval x env)))
-  :fn width-of-svex
+(local
+ (defthm car-of-assoc-equal
+   (implies (assoc-equal fn alist)
+            (equal (car (assoc-equal fn alist))
+                   fn))))
+
+(defthm width-of-svex-extn-p-of-assoc-equal-of-svex-functions
+  (implies (assoc-equal fn sv::*svex-op-table*)
+           (not (width-of-svex-extn-p (assoc-equal fn extensions))))
   :hints (("goal"
-           :expand ((:free (fn x y)
-                           (svex-apply fn (cons x y)))
-                    (svexlist-eval (svex-call->args x)
-                                   env)
-                    (svexlist-eval (cdr (svex-call->args x))
-                                   env)
-                    (svexlist-eval (cddr (svex-call->args x))
-                                   env)
-                    (svexlist-eval (cdddr (svex-call->args x))
-                                   env))
-           :in-theory (e/d (svex-p
-                            nfix
-                            ;;4vec-part-install
-                            4vec-concat$
-                            width-of-svex
-                            4vec-part-select-of-4vec-bitxor-better
-                            4vec-part-select-of-4vec-bitor-better
-                            4vec-part-select-of-4vec-bitand-better
-                            svexlist-eval
-                            4vec-part-select-of-4vec-bit?!-2
-                            4vec-part-select-of-4vec-bit?-2)
-                           (loghead
-                            logapp
-                            4vec-part-select-of-4vec-bit?!
-                            4vec-part-select-of-4vec-bit?)))
-          (and stable-under-simplificationp
-               '(:use ((:instance svex-eval-<fn>-is-correct-when-quoted)))))))
+           :cases ((assoc-equal fn extensions))
+           :in-theory (e/d
+                       (svex-foreign-fnsym-p
+                        width-of-svex-extn-p)
+                       (assoc-equal)))))
+
+(local
+ (defthm 4vec-correct-width-p-of-not-natp
+   (implies (not (natp width))
+            (4vec-correct-width-p width x))
+   :hints (("goal"
+            :in-theory (e/d (4vec-correct-width-p) ())))))
+
+
+
+
+(local
+ (defthm 4vec-correct-width-p-expand
+   (implies (syntaxp (and (consp term)
+                          (assoc-equal (car term)
+                                       (strip-cdrs sv::*svex-op-table*))))
+            (equal (4vec-correct-width-p width term)
+                   (implies (natp width)
+                            (equal (4vec-part-select 0 width term)
+                                   term))))
+   :hints (("goal"
+            :in-theory (e/d (4vec-correct-width-p) ())))))
+
+(local
+ (defthm 4vec-correct-width-p-of-and
+   (equal (4vec-correct-width-p (and x y) val)
+          (implies x
+                   (4vec-correct-width-p y val)))))
+
+(local
+ (defthm width-of-svex-extn-correct$-of-assoc
+   (implies (and (assoc-equal fn extns)
+                 (width-of-svex-extn-correct$-lst extns))
+            (width-of-svex-extn-correct$
+             (assoc-equal fn extns)))
+   :hints (("goal"
+            :in-theory (e/d () (width-of-svex-extn-correct$))))))
+
+(defret len-of-widths-of-svexlist
+  (equal (len widths)
+         (len lst))
+  :fn widths-of-svexlist
+  :hints (("goal"
+           :induct (len lst)
+           :in-theory (e/d (widths-of-svexlist) ()))))
+
+(local
+ (defthm width-of-svex-extn->fn-of-assoc-equal
+   (implies (and (width-of-svex-extn-p (assoc-equal fn lst)))
+            (equal (width-of-svex-extn->fn (assoc-equal fn lst))
+                   fn))
+   :hints (("goal"
+            :in-theory (e/d (width-of-svex-extn-p
+                             width-of-svex-extn->fn) ())))))
+
+(local
+ (defthm 4vec-correct-width-p-of-width-of-svex-extn-formula-eval
+   (implies (and (width-of-svex-extn-correct$ extn)
+                 (4vec-correct-widths-p arg-widths (svexlist-eval$ args env))
+                 (equal (len args)
+                        (width-of-svex-extn->arg-len extn))
+                 (equal (len args) (len arg-widths))
+                 (equal fn (width-of-svex-extn->fn extn))
+                 (width-of-svex-extn-p extn)
+                 ;;(not (member-equal fn (strip-cars sv::*svex-op-table*)))
+                 )
+            (4vec-correct-width-p
+             (width-of-svex-extn-formula-eval
+              (width-of-svex-extn->formula extn)
+              arg-widths)
+             (svex-apply$ fn (svexlist-eval$ args env))))
+   :hints (("goal"
+            :do-not-induct t
+            :use ((:instance width-of-svex-extn-correct$-necc
+                             (widths arg-widths)
+                             (obj extn)))
+            :in-theory (e/d ()
+                            (width-of-svex-extn-correct$
+                             width-of-svex-extn-correct$-necc))))))
+
+(local
+ (svex-eval-lemma-tmpl
+  (defthm svex-apply-opener-for-known-functions
+    (implies (not (svex-foreign-fnsym-p fn))
+             (equal (svex-apply fn args)
+                    (let* ((fn (fnsym-fix fn))
+                           (args (sv::4veclist-fix args)))
+                      (svex-apply-cases fn args))))
+    :hints (("goal"
+             :in-theory (e/d (svex-apply) ()))))))
+
+(local
+ (in-theory (disable SV::SVEXLIST-EVAL$-IS-SVEXLIST-EVAL)))
+
+(svex-eval-lemma-tmpl
+ (defret-mutual svex-eval-width-is-correct-1
+   (defret svex-eval-<fn>-is-correct-1
+     (implies (and ;;width
+               (sv::Svex-p x)
+               (:@ :dollar-eval
+                   (width-of-svex-extn-correct<$>-lst
+                    (svex-reduce-config->width-extns config)))
+               (:@ :normal-eval
+                   (equal (svex-reduce-config->width-extns config) nil)))
+              (4vec-correct-width-p width (svex-eval x env))
+              #|(equal (4vec-part-select 0 width (svex-eval x env))
+              (svex-eval x env))|#)
+     :fn width-of-svex)
+   (defret svexlist-eval-<fn>-is-correct-1
+     (implies (and ;;widths
+               (sv::Svexlist-p lst)
+               (:@ :dollar-eval
+                   (width-of-svex-extn-correct<$>-lst
+                    (svex-reduce-config->width-extns config)))
+               (:@ :normal-eval
+                   (equal (svex-reduce-config->width-extns config) nil)))
+              (and
+               ;;(equal (len lst) (len widths))
+               (4vec-correct-widths-p widths
+                                      (svexlist-eval lst env))))
+     :fn widths-of-svexlist)
+   ;;:otf-flg t
+   :hints (("goal"
+            :do-not-induct t
+            :expand ((:free (x y z)
+                            (4VEC-CORRECT-WIDTHS-P (cons x y) z))
+                     (:free (x y)
+                            (len (cons x y)))
+                     (4vec-correct-width-p (width-of-svex (car (svex-call->args x)))
+                                           (svex-eval (car (svex-call->args x))
+                                                      env))
+                     (4vec-correct-width-p (width-of-svex (cadr (svex-call->args x)))
+                                           (svex-eval (cadr (svex-call->args x))
+                                                      env))
+                     (4vec-correct-width-p (width-of-svex (caddr (svex-call->args x)))
+                                           (svex-eval (caddr (svex-call->args x))
+                                                      env))
+                     (4vec-correct-width-p 0
+                                           (svex-eval (caddr (svex-call->args x))
+                                                      env))
+                     (4vec-correct-width-p (integer-length x)
+                                           x)
+
+                     (widths-of-svexlist nil)
+                     (widths-of-svexlist lst)
+
+                     #|(:free (fn x y)
+                     (svex-apply fn (cons x y)))|#
+                     ;; (svexlist-eval (svex-call->args x)
+                     ;;                env)
+                     ;; (svexlist-eval (cdr (svex-call->args x))
+                     ;;                env)
+                     ;; (svexlist-eval (cddr (svex-call->args x))
+                     ;;                env)
+                     ;; (svexlist-eval (cdddr (svex-call->args x))
+                     ;;                env)
+                     )
+            :in-theory (e/d (;;4vec-correct-widths-p
+                             ;;4vec-correct-width-p
+                             or*
+                             len
+                             svex-p
+                             nfix
+                             ;;4vec-part-install
+                             4vec-concat$
+                             width-of-svex
+                             ;;widths-of-svexlist
+                             4vec-part-select-of-4vec-bitxor-better
+                             4vec-part-select-of-4vec-bitor-better
+                             4vec-part-select-of-4vec-bitand-better
+                             svexlist-eval
+                             4vec-part-select-of-4vec-bit?!-2
+                             4vec-part-select-of-4vec-bit?-2
+
+                             )
+                            (
+                             (:definition svex-p)
+                             (:rewrite default-<-1)
+                             (:rewrite default-<-2)
+
+                             svex-apply
+                             (:rewrite default-cdr)
+                             (:rewrite default-car)
+                             ;;(:definition assoc-equal)
+                             (:meta
+                              rp::binary-or**/and**-guard-meta-correct)
+                             ;;(:rewrite dummy-lemma-1)
+
+                             (:type-prescription
+                              posp-of-width-of-svex-extn->arg-len)
+                             (:type-prescription len)
+                             ;;(:definition len)
+                             (:definition member-equal)
+                             width-of-svex-extn-correct$
+                             rp::len-cons
+                             acl2::equal-len-1
+                             rp::dummy-len-equiv
+                             loghead
+                             logapp
+                             4vec-part-select-of-4vec-bit?!
+                             4vec-part-select-of-4vec-bit?)))
+           (and stable-under-simplificationp
+                '(:expand ((svexlist-eval (svex-call->args x)
+                                          env)
+                           (svexlist-eval (cdr (svex-call->args x))
+                                          env)
+                           (svexlist-eval (cddr (svex-call->args x))
+                                          env)
+                           (svexlist-eval (cdddr (svex-call->args x))
+                                          env))
+                          :use ((:instance svex-eval-width-of-svex-is-correct-when-quoted)))))))
 
 (svex-eval-lemma-tmpl
  (defret svex-eval-<fn>-is-correct
-  (implies (and width
-                (equal free-var-width width)
-                (sv::Svex-p x))
-           (equal (4vec-part-select 0 free-var-width (svex-eval x env))
-                  (svex-eval x env)))
-  :fn width-of-svex))
+   (implies (and width
+                 (equal free-var-width width)
+                 (sv::svex-p x)
+                 (:@ :dollar-eval
+                     (width-of-svex-extn-correct<$>-lst
+                      (svex-reduce-config->width-extns config)))
+                 (:@ :normal-eval
+                     (equal (svex-reduce-config->width-extns config) nil)))
+            (and (equal (4vec-part-select 0 free-var-width (svex-eval x env))
+                        (svex-eval x env))
+                 (4vec-correct-width-p free-var-width (svex-eval x env))))
+   :fn width-of-svex
+   :hints (("goal"
+            :use ((:instance svex-eval-width-of-svex-is-correct-1))
+            :in-theory (e/d (4vec-correct-width-p) ())))))
+
+
+;; (width-of-svex '(ha-s (partsel 0 2 a) (partsel 0 3 a))
+;;                :config (make-svex-reduce-config
+;;                         :width-extns (list
+;;                                       (make-width-of-svex-extn
+;;                                        :fn 'ha-s
+;;                                        :arg-len 2
+;;                                        :formula '(safe-max (nth '0 widths)
+;;                                                            (nth '1 widths))))))
+;; returns
+;; 3. 
+                                      
